revm:add clone for EofBody

CoqOfRust/alloc/vec/links/mod.v
@@ -4,15 +4,40 @@ Require Import links.M.
 Import Run.
 
 Module Vec.
-  Record t {A : Set} : Set := {
-    value : list A;
+  Record t {T A : Set} : Set := {
+    value : list T;
   }.
   Arguments t : clear implicits.
 
-  Parameter to_value : forall {A : Set}, t A -> Value.t.
+  Parameter to_value : forall {T A : Set}, t T A -> Value.t.
 
-  Global Instance IsLink (A : Set) (_ : Link A) : Link (t A) := {
-    Φ := Ty.apply (Ty.path "vec") [] [Φ A];
+  Global Instance IsLink (T A : Set) `(Link T) `(Link A) : Link (t T A) := {
+    Φ := Ty.apply (Ty.path "alloc::vec::Vec") [] [Φ T; Φ A];
     φ := to_value;
   }.
+
+  Definition of_ty (T' A' : Ty.t) : 
+    OfTy.t T' ->
+    OfTy.t A' ->
+    OfTy.t (Ty.apply (Ty.path "alloc::vec::Vec") [] [T'; A']).
+  Proof. 
+    intros [T] [A].
+    eapply OfTy.Make with (A := t T A). 
+    subst.
+    reflexivity. 
+  Defined.
+  Smpl Add apply of_ty : of_ty.
 End Vec.
+
+Module Impl_Clone_for_Vec.
+  Definition run_clone {T A : Set} `{Link T} `{Link A} : clone.Clone.Run_clone (Vec.t T A).
+  Admitted.
+
+  Definition run {T A : Set} `{Link T} `{Link A} : clone.Clone.Run (Vec.t T A).
+  Proof.
+    constructor.
+    { (* clone *)
+      exact run_clone.
+    }
+  Defined.
+End Impl_Clone_for_Vec.
