CoqOfRust/revm/revm_bytecode/eof/links/types_section.v
@@ -1,7 +1,7 @@
 Require Import CoqOfRust.CoqOfRust.
 Require Import links.M.
 Require alloc.links.alloc.
-Require alloc.links.vec.
+Require alloc.vec.links.mod.
 Require Import revm.links.dependencies.
 
 Module TypesSection.
@@ -20,4 +20,8 @@ Module TypesSection.
         ("max_stack_size", φ max_stack_size)
       ]
   }.
+
+  Definition of_ty : OfTy.t (Ty.path "revm_bytecode::eof::types_section::TypesSection").
+  Proof. eapply OfTy.Make with (A := t); reflexivity. Defined.
+  Smpl Add apply of_ty : of_ty.
 End TypesSection.
